More region work (ultimately doesn't work)
git-svn-id: orca@492

C-verifier/src/Midend-IVL/Isabelle-UTP-Extended/dev_work/TotalCorrectness/Rel/framing.thy
@@ -6,7 +6,225 @@ imports
   "../../../utils/vcg_helpers"
 begin
 
-text \<open>Using locales for modularity\<close>
+definition \<open>EXINV l P \<equiv> \<^bold>\<exists>st \<bullet> P\<lbrakk>(\<guillemotleft>st\<guillemotright> \<oplus> &\<Sigma> on &l)/&\<Sigma>\<rbrakk>\<close>
+
+subsection \<open>Modification is existential\<close>
+
+definition \<open>modifies x \<equiv> \<^bold>\<exists>v' \<bullet> $\<Sigma>\<acute> \<oplus> \<guillemotleft>v'\<guillemotright> on &x =\<^sub>u $\<Sigma>\<close>
+
+lemma modifies_to_ext:
+  assumes \<open>vwb_lens x\<close>
+      and \<open>modifies x \<sqsubseteq> c\<close>
+  shows \<open>\<lbrace>P\<rbrace>c\<lbrace>\<exists>x \<bullet> P\<rbrace>\<^sub>u\<close>
+  using assms unfolding modifies_def
+  by rel_simp metis
+
+lemma ext_to_modifies:
+  assumes \<open>vwb_lens x\<close>
+      and \<open>\<forall>P. \<lbrace>P\<rbrace>c\<lbrace>\<exists>x \<bullet> P\<rbrace>\<^sub>u\<close>
+  shows \<open>modifies x \<sqsubseteq> c\<close>
+  using assms unfolding modifies_def
+  apply - \<comment> \<open>Why do we need to inline the assumptions? Weird.\<close>
+  apply rel_simp
+  by (metis skip_r_eq subst.rep_eq vwb_lens.put_eq)
+
+lemma modifies_ext:
+  assumes \<open>vwb_lens x\<close>
+  shows \<open>modifies x \<sqsubseteq> c = (\<forall>P. \<lbrace>P\<rbrace>c\<lbrace>\<exists>x \<bullet> P\<rbrace>\<^sub>u)\<close>
+  by (metis assms modifies_to_ext ext_to_modifies)
+
+subsection \<open>Region-based modifies\<close>
+text \<open>We want to be able to reason about the intersection of lenses and the above modifies does not
+allow us to do so.\<close>
+
+definition region :: \<open>('a \<Longrightarrow> '\<alpha>) \<Rightarrow> '\<alpha> \<Rightarrow> '\<alpha> set\<close> where
+  \<open>region x s = {s'. \<exists>v. s' = put\<^bsub>x\<^esub> s v}\<close>
+
+definition region_modifies :: \<open>('\<alpha> \<Rightarrow> '\<alpha> set) \<Rightarrow> _\<close> where
+  \<open>region_modifies reg \<equiv> $\<Sigma>\<acute> \<in>\<^sub>u uop reg $\<Sigma>\<close>
+
+abbreviation region_modifies_ref where
+  \<open>region_modifies_ref r c \<equiv> region_modifies r \<sqsubseteq> c\<close>
+
+lemma region_modifies_to_ext:
+  assumes \<open>region_modifies (region x) \<sqsubseteq> c\<close>
+          \<open>vwb_lens x\<close>
+  shows \<open>\<lbrace>P\<rbrace>c\<lbrace>\<exists>x \<bullet> P\<rbrace>\<^sub>u\<close>
+  using assms unfolding region_modifies_def region_def
+  by rel_simp (metis vwb_lens.put_eq)
+
+lemma ext_to_region_modifies:
+  assumes \<open>\<forall>P. \<lbrace>P\<rbrace>c\<lbrace>\<exists>x \<bullet> P\<rbrace>\<^sub>u\<close>
+          \<open>vwb_lens x\<close>
+  shows \<open>region_modifies (region x) \<sqsubseteq> c\<close>
+  using assms unfolding region_modifies_def region_def
+  by rel_simp (metis (no_types, hide_lams) skip_r_eq subst.rep_eq vwb_lens.put_eq)
+
+lemma region_modifies_ext:
+  assumes \<open>vwb_lens x\<close>
+  shows \<open>region_modifies (region x) \<sqsubseteq> c = (\<forall>P. \<lbrace>P\<rbrace>c\<lbrace>\<exists>x \<bullet> P\<rbrace>\<^sub>u)\<close>
+  using assms ext_to_region_modifies region_modifies_to_ext
+  by blast
+
+text \<open>supposed to be @{text \<sqinter>} but UTP messed it up\<close>
+abbreviation \<open>reg_inter r\<^sub>1 r\<^sub>2 \<equiv> Lattices.inf r\<^sub>1 r\<^sub>2\<close> \<comment> \<open>@{text \<open>\<lambda>s. r\<^sub>1 s \<inter> r\<^sub>2 s\<close>}\<close>
+
+lemma reg_mod_intersect: \<comment> \<open>Greatest lower bound\<close>
+  assumes \<open>region_modifies r\<^sub>1 \<sqsubseteq> c\<close> \<open>region_modifies r\<^sub>2 \<sqsubseteq> c\<close>
+  shows \<open>region_modifies (reg_inter r\<^sub>1 r\<^sub>2) \<sqsubseteq> c\<close>
+  using assms unfolding region_def region_modifies_def
+  by rel_simp
+
+lemma reg_mod_intersect_sym:
+  assumes \<open>region_modifies (reg_inter r\<^sub>1 r\<^sub>2) \<sqsubseteq> c\<close>
+  shows \<open>region_modifies r\<^sub>1 \<sqsubseteq> c\<close> \<open>region_modifies r\<^sub>2 \<sqsubseteq> c\<close> \<comment> \<open>@{text \<ge>}\<close>
+  using assms unfolding region_def region_modifies_def
+  by rel_simp+
+
+lemma reg_mod_intersect_antiframe1: (* This works but does it actually help? *)
+  assumes \<open>region_modifies r\<^sub>1 \<sqsubseteq> c\<close> \<open>region_modifies r\<^sub>2 \<sqsubseteq> c\<close>
+          \<open>vwb_lens b\<close>
+  shows \<open>region_modifies (reg_inter r\<^sub>1 r\<^sub>2) \<sqsubseteq> b:[c]\<close>
+  using assms unfolding region_modifies_def region_def
+  apply rel_auto
+    oops
+   apply (metis mwb_lens.put_put vwb_lens_def wb_lens.get_put)
+  apply (metis vwb_lens.put_eq)
+  done
+
+lemma reg_mod_intersect_antiframe2:
+  assumes \<open>region_modifies r\<^sub>1 \<sqsubseteq> c\<close> \<open>region_modifies r\<^sub>2 \<sqsubseteq> c\<close>
+          \<open>vwb_lens a\<close>
+  shows \<open>region_modifies (reg_inter r\<^sub>1 r\<^sub>2) \<sqsubseteq> a:[c]\<close>
+  using assms unfolding region_modifies_def region_def
+  apply rel_auto
+  oops
+    apply (metis vwb_lens_def wb_lens.get_put)
+  apply (metis vwb_lens.put_eq)
+  done
+
+subsection \<open>Regions of a program\<close>
+
+definition \<open>prog_region c s = {s'. \<lbrakk>c\<rbrakk>\<^sub>e (s, s')}\<close>
+abbreviation prog_region_ref (infix "\<flat>" 95) where
+  \<open>r \<flat> c \<equiv> r \<ge> prog_region c\<close>
+
+lemma reg_mod_prog_temp:
+  \<open>region_modifies r \<sqsubseteq> c = r \<flat> c\<close>
+  unfolding prog_region_def region_modifies_def
+  by rel_auto (auto simp: le_fun_def)
+
+lemma prog_reg_to_ext:
+  assumes \<open>region x \<flat> c\<close>
+          \<open>vwb_lens x\<close>
+  shows \<open>\<lbrace>P\<rbrace>c\<lbrace>\<exists>x \<bullet> P\<rbrace>\<^sub>u\<close>
+proof -
+  have \<open>(region x) \<flat> c = (\<forall>s s'. \<lbrakk>c\<rbrakk>\<^sub>e (s, s') \<longrightarrow> (\<exists>v. s' = put\<^bsub>x\<^esub> s v))\<close>
+    unfolding prog_region_def region_def le_fun_def
+    by auto
+  with assms show ?thesis by rel_simp (metis vwb_lens.put_eq)
+qed
+  
+lemma ext_to_prog_reg:
+  assumes \<open>\<forall>P. \<lbrace>P\<rbrace>c\<lbrace>\<exists>x \<bullet> P\<rbrace>\<^sub>u\<close>
+          \<open>vwb_lens x\<close>
+  shows \<open>region x \<flat> c\<close>
+  using assms unfolding prog_region_def region_def le_fun_def
+  by rel_simp (metis (no_types, hide_lams) skip_r_eq subst.rep_eq vwb_lens.put_eq)
+
+lemma prog_reg_ext:
+  assumes \<open>vwb_lens x\<close>
+  shows \<open>(region x) \<flat> c = (\<forall>P. \<lbrace>P\<rbrace>c\<lbrace>\<exists>x \<bullet> P\<rbrace>\<^sub>u)\<close>
+  using assms prog_reg_to_ext ext_to_prog_reg
+  by blast
+
+lemma prog_reg_inf_antiframe:
+  assumes \<open>r \<flat> c\<close>
+          \<open>vwb_lens x\<close>
+  shows \<open>reg_inter r (region x) \<flat> x:[c]\<close>
+  using assms unfolding prog_region_def region_def le_fun_def
+  apply rel_auto
+  oops
+
+text \<open>Lenses are too abstract for proper region reasoning right now.\<close>
+
+subsection \<open>Antiframe rule work\<close>
+
+lemma antiframe_rule[hoare_rules]:
+  assumes \<open>vwb_lens a\<close> \<open>\<lbrace>P\<rbrace>c\<lbrace>Q\<rbrace>\<^sub>u\<close>
+  shows \<open>\<lbrace>P\<rbrace> a:[c] \<lbrace>(\<exists>a \<bullet> P) \<and> (EXINV a Q)\<rbrace>\<^sub>u\<close>
+  using assms unfolding EXINV_def
+  by rel_simp (metis assms(1) vwb_lens_wb wb_lens.get_put)
+
+declare assigns_floyd_r[hoare_rules del]
+lemma assigns_floyd_rX [hoare_rules]:
+  assumes \<open>vwb_lens x\<close>
+  shows   \<open>\<lbrace>p\<rbrace>x :== e\<lbrace>(\<exists>x \<bullet> p) \<and> (\<^bold>\<exists>v \<bullet> &x =\<^sub>u e\<lbrakk>\<guillemotleft>v\<guillemotright>/x\<rbrakk>)\<rbrace>\<^sub>u\<close>
+  apply (insert assms)
+  apply pred_simp
+  apply transfer
+  apply rule
+   apply (rule_tac x = \<open>get\<^bsub>x\<^esub> a\<close> in exI)
+   apply auto
+  apply (rule_tac x = \<open>get\<^bsub>x\<^esub> a\<close> in exI)
+  apply auto
+  done
+
+lemma modified_assign_rule:
+  assumes \<open>vwb_lens x\<close>
+  shows   \<open>\<lbrace>p\<rbrace>x :== e\<lbrace>(\<exists>x \<bullet> p)\<rbrace>\<^sub>u\<close>
+  apply (rule hoare_post_weak)
+   apply (rule assigns_floyd_rX)
+   apply fact
+  apply pred_simp
+  done
+
+lemma EXINV_pull_out_sublens:
+  assumes A: \<open>vwb_lens x\<close> \<open>vwb_lens l\<close>
+  defines \<open>XX \<equiv> x ;\<^sub>L l\<close>
+  shows \<open>EXINV l (\<exists>XX \<bullet> P) = (\<exists>XX \<bullet> EXINV l P)\<close>
+  unfolding EXINV_def XX_def using A
+  by pred_blast
+
+lemma EXINV_drop_indep:
+  assumes A: \<open>vwb_lens l\<^sub>1\<close> \<open>vwb_lens l\<^sub>2\<close> \<open>l\<^sub>1 \<bowtie> l\<^sub>2\<close>
+  shows "EXINV l\<^sub>1 (\<exists>l\<^sub>2 \<bullet> P) = (EXINV l\<^sub>1 P)"
+  unfolding EXINV_def using A
+  by pred_simp (metis lens_indep_def vwb_lens_wb wb_lens.get_put)
+
+lemma lens_indep_right_ext' [intro, simp]:
+  \<open>z \<bowtie> x \<Longrightarrow> x \<bowtie> (y ;\<^sub>L z)\<close>
+  using lens_indep_sym by blast
+
+lemma lens_indep_left_ext' [intro, simp]:
+  \<open>x \<bowtie> z \<Longrightarrow> (y ;\<^sub>L z) \<bowtie> x\<close>
+  using lens_indep_sym by blast
+
+(*lemmas [simp] = lens_indep_right_ext lens_indep_left_ext*)
+
+lemma conj_ex2_move_front: \<open>l \<sharp> P \<Longrightarrow> (P \<and> (\<exists>l \<bullet> Q)) = (\<exists>l \<bullet> P \<and> Q)\<close>
+  by pred_simp
+
+lemma dep_unrest_ex:
+  assumes A: \<open>vwb_lens x\<close> \<open>vwb_lens l\<close>
+  defines \<open>XX \<equiv> x;\<^sub>Ll\<close>
+  shows \<open>XX \<sharp> (\<exists> l \<bullet> F)\<close>
+  unfolding XX_def using A
+  by pred_simp
+
+lemma
+  assumes \<open>vwb_lens l\<close>
+  shows \<open>((\<exists> l \<bullet> F) \<and> EXINV l F) = F\<close>
+  using assms
+  unfolding EXINV_def
+  apply pred_simp
+  apply transfer
+  oops
+
+lemma \<open>(\<exists>x. P x y) \<and> (\<exists>y. P x y) \<Longrightarrow> P x y\<close>
+  oops
+
+subsection \<open>Locales for modularity\<close>
 
 locale peter =
   fixes lvars :: \<open>'l \<Longrightarrow> 's\<close>
@@ -17,6 +235,7 @@ locale peter =
   assumes INDEP: \<open>lvars \<bowtie> gvars\<close> \<open>x \<bowtie> y\<close>
           \<open>vwb_lens lvars\<close> \<open>vwb_lens gvars\<close> \<open>vwb_lens ret\<close> \<open>vwb_lens x\<close> \<open>vwb_lens y\<close>
 begin
+
 abbreviation \<open>Lx \<equiv> x ;\<^sub>L lvars\<close>
 abbreviation \<open>Ly \<equiv> y ;\<^sub>L lvars\<close>
 abbreviation \<open>Gret \<equiv> ret ;\<^sub>L gvars\<close>
@@ -31,168 +250,6 @@ lemma f_rule:
   shows \<open>\<lbrace> e=\<^sub>u\<guillemotleft>val\<guillemotright> \<rbrace> f r e \<lbrace> &r=\<^sub>u\<guillemotleft>val+1\<guillemotright> \<rbrace>\<^sub>u\<close>
   unfolding f_def using assms INDEP
   by rel_simp
-
-definition (in -) \<open>EXINV l P \<equiv> \<^bold>\<exists>st \<bullet> P\<lbrakk>(\<guillemotleft>st\<guillemotright> \<oplus> &\<Sigma> on &l)/&\<Sigma>\<rbrakk>\<close>
-
-subsection \<open>Modification is existential\<close>
-
-definition (in -) \<open>modifies x \<equiv> \<^bold>\<exists>v' \<bullet> $\<Sigma>\<acute> \<oplus> \<guillemotleft>v'\<guillemotright> on &x =\<^sub>u $\<Sigma>\<close>
-abbreviation (in -) ref_modifies (infix "\<flat>" 95) where
-  \<open>x \<flat> c \<equiv> modifies x \<sqsubseteq> c\<close>
-
-lemma (in -) modifies_to_ext:
-  assumes \<open>vwb_lens x\<close>
-      and \<open>modifies x \<sqsubseteq> c\<close> (* TODO: use notation? *)
-  shows \<open>\<lbrace>P\<rbrace>c\<lbrace>\<exists>x \<bullet> P\<rbrace>\<^sub>u\<close>
-  using assms unfolding modifies_def
-  by rel_simp metis
-
-lemma (in -) ext_to_modifies:
-  assumes \<open>vwb_lens x\<close>
-      and \<open>\<forall>P. \<lbrace>P\<rbrace>c\<lbrace>\<exists>x \<bullet> P\<rbrace>\<^sub>u\<close>
-  shows \<open>modifies x \<sqsubseteq> c\<close>
-  using assms unfolding modifies_def
-  apply - \<comment> \<open>Why do we need to inline the assumptions? Weird.\<close>
-  apply rel_simp
-  by (metis skip_r_eq subst.rep_eq vwb_lens.put_eq)
-
-lemma (in -) modifies_ext:
-  assumes \<open>vwb_lens x\<close>
-  shows \<open>modifies x \<sqsubseteq> c = (\<forall>P. \<lbrace>P\<rbrace>c\<lbrace>\<exists>x \<bullet> P\<rbrace>\<^sub>u)\<close>
-  by (metis assms modifies_to_ext ext_to_modifies)
-
-subsection \<open>Region-based modifies\<close>
-
-definition (in -) region :: \<open>('a \<Longrightarrow> '\<alpha>) \<Rightarrow> '\<alpha> \<Rightarrow> '\<alpha> set\<close> where
-  \<open>region x s = {s'. \<exists>v. s = put\<^bsub>x\<^esub> s' v}\<close>
-
-definition (in -) region_modifies :: \<open>('\<alpha> \<Rightarrow> '\<alpha> set) \<Rightarrow> _\<close> where
-  \<open>region_modifies reg \<equiv> $\<Sigma>\<acute> \<in>\<^sub>u uop reg $\<Sigma>\<close>
-
-lemma (in -) region_modifies_to_ext:
-  assumes \<open>region_modifies (region x) \<sqsubseteq> c\<close>
-  shows \<open>\<lbrace>P\<rbrace>c\<lbrace>\<exists>x \<bullet> P\<rbrace>\<^sub>u\<close>
-  using assms unfolding region_modifies_def region_def
-  by rel_simp blast
-
-lemma (in -) ext_to_region_modifies:
-  assumes \<open>\<forall>P. \<lbrace>P\<rbrace>c\<lbrace>\<exists>x \<bullet> P\<rbrace>\<^sub>u\<close>
-  shows \<open>region_modifies (region x) \<sqsubseteq> c\<close>
-  using assms unfolding region_modifies_def region_def
-  by rel_simp (metis skip_r_eq subst.rep_eq)
-
-lemma (in -) region_modifies_ext:
-  \<open>region_modifies (region x) \<sqsubseteq> c = (\<forall>P. \<lbrace>P\<rbrace>c\<lbrace>\<exists>x \<bullet> P\<rbrace>\<^sub>u)\<close>
-  using ext_to_region_modifies region_modifies_to_ext
-  by blast
-
-abbreviation
-  \<open>reg_mod_intersect a b \<equiv> region_modifies (\<lambda>s. region a s \<inter> region b s)\<close>
-
-lemma reg_mod_intersect:
-  assumes \<open>region_modifies (region a) \<sqsubseteq> c\<close>
-          \<open>region_modifies (region b) \<sqsubseteq> c\<close>
-  shows \<open>reg_mod_intersect a b \<sqsubseteq> c\<close>
-  using assms unfolding region_def region_modifies_def
-  by rel_simp
-
-lemma reg_mod_intersect_antiframe1: (* This works but does it actually help? *)
-  assumes \<open>region_modifies (region a) \<sqsubseteq> c\<close>
-          \<open>region_modifies (region b) \<sqsubseteq> c\<close>
-          \<open>vwb_lens b\<close>
-  shows \<open>reg_mod_intersect a b \<sqsubseteq> b:[c]\<close>
-  using assms unfolding region_modifies_def region_def
-  apply rel_auto
-   apply (metis mwb_lens.put_put vwb_lens_def wb_lens.get_put)
-  apply (metis vwb_lens.put_eq)
-  done
-
-lemma reg_mod_intersect_antiframe2:
-  assumes \<open>region_modifies (region a) \<sqsubseteq> c\<close>
-          \<open>region_modifies (region b) \<sqsubseteq> c\<close>
-          \<open>vwb_lens a\<close>
-  shows \<open>reg_mod_intersect a b \<sqsubseteq> a:[c]\<close>
-  using assms unfolding region_modifies_def region_def
-  apply rel_auto
-   apply (metis vwb_lens_def wb_lens.get_put)
-  apply (metis vwb_lens.put_eq)
-  done
-
-subsection \<open>Antiframe rule work\<close>
-
-lemma antiframe_rule[hoare_rules]:
-  assumes \<open>vwb_lens a\<close> \<open>\<lbrace>P\<rbrace>c\<lbrace>Q\<rbrace>\<^sub>u\<close>
-  shows \<open>\<lbrace>P\<rbrace> a:[c] \<lbrace>(\<exists>a \<bullet> P) \<and> (EXINV a Q)\<rbrace>\<^sub>u\<close>
-  using assms unfolding EXINV_def
-  by rel_simp (metis assms(1) vwb_lens_wb wb_lens.get_put)
-
-declare assigns_floyd_r[hoare_rules del]
-lemma (in -) assigns_floyd_rX [hoare_rules]:
-  assumes \<open>vwb_lens x\<close>
-  shows   \<open>\<lbrace>p\<rbrace>x :== e\<lbrace>(\<exists>x \<bullet> p) \<and> (\<^bold>\<exists>v \<bullet> &x =\<^sub>u e\<lbrakk>\<guillemotleft>v\<guillemotright>/x\<rbrakk>)\<rbrace>\<^sub>u\<close>
-  apply (insert assms)
-  apply pred_simp
-  apply transfer
-  apply rule
-   apply (rule_tac x = \<open>get\<^bsub>x\<^esub> a\<close> in exI)
-   apply auto
-  apply (rule_tac x = \<open>get\<^bsub>x\<^esub> a\<close> in exI)
-  apply auto
-  done
-
-lemma (in -) modified_assign_rule:
-  assumes \<open>vwb_lens x\<close>
-  shows   \<open>\<lbrace>p\<rbrace>x :== e\<lbrace>(\<exists>x \<bullet> p)\<rbrace>\<^sub>u\<close>
-  apply (rule hoare_post_weak)
-   apply (rule assigns_floyd_rX)
-   apply fact
-  apply pred_simp
-  done
-
-lemma (in -) EXINV_pull_out_sublens:
-  assumes A: \<open>vwb_lens x\<close> \<open>vwb_lens l\<close>
-  defines \<open>XX \<equiv> x ;\<^sub>L l\<close>
-  shows \<open>EXINV l (\<exists>XX \<bullet> P) = (\<exists>XX \<bullet> EXINV l P)\<close>
-  unfolding EXINV_def XX_def using A
-  by pred_blast
-
-lemma (in -) EXINV_drop_indep:
-  assumes A: \<open>vwb_lens l\<^sub>1\<close> \<open>vwb_lens l\<^sub>2\<close> \<open>l\<^sub>1 \<bowtie> l\<^sub>2\<close>
-  shows "EXINV l\<^sub>1 (\<exists>l\<^sub>2 \<bullet> P) = (EXINV l\<^sub>1 P)"
-  unfolding EXINV_def using A
-  by pred_simp (metis lens_indep_def vwb_lens_wb wb_lens.get_put)
-
-lemma (in -) lens_indep_right_ext' [intro, simp]:
-  \<open>z \<bowtie> x \<Longrightarrow> x \<bowtie> (y ;\<^sub>L z)\<close>
-  using lens_indep_sym by blast
-
-lemma (in -) lens_indep_left_ext' [intro, simp]:
-  \<open>x \<bowtie> z \<Longrightarrow> (y ;\<^sub>L z) \<bowtie> x\<close>
-  using lens_indep_sym by blast
-
-(*lemmas [simp] = lens_indep_right_ext lens_indep_left_ext*)
-
-lemma conj_ex2_move_front: \<open>l \<sharp> P \<Longrightarrow> (P \<and> (\<exists>l \<bullet> Q)) = (\<exists>l \<bullet> P \<and> Q)\<close>
-  by pred_simp
-
-lemma (in -) dep_unrest_ex:
-  assumes A: \<open>vwb_lens x\<close> \<open>vwb_lens l\<close>
-  defines \<open>XX \<equiv> x;\<^sub>Ll\<close>
-  shows \<open>XX \<sharp> (\<exists> l \<bullet> F)\<close>
-  unfolding XX_def using A
-  by pred_simp
-
-lemma (in -)
-  assumes \<open>vwb_lens l\<close>
-  shows \<open>((\<exists> l \<bullet> F) \<and> EXINV l F) = F\<close>
-  using assms
-  unfolding EXINV_def
-  apply pred_simp
-  apply transfer
-  oops
-
-lemma (in -) \<open>(\<exists>x. P x y) \<and> (\<exists>y. P x y) \<Longrightarrow> P x y\<close>
-  oops
 
 lemma
   assumes \<open>vwb_lens r\<close>
@@ -218,8 +275,6 @@ lemma
   apply solve_vcg
   apply pred_simp
   apply (simp add: vwb_lens_wb[THEN wb_lens.get_put])
-
-
 
 end
 
